theories/Block/vst/verif/certicoq_block__field_iter.v
@@ -1,0 +1,14 @@
+From VST Require Import floyd.proofauto.
+
+From CertiCoq Require Import Block.vst.ast.ast.
+From CertiCoq Require Import Block.vst.clightgen.block.
+From CertiCoq Require Import Block.vst.cmodel.certicoq_block_header.
+From CertiCoq Require Import Block.vst.cmodel.certicoq_block.
+From CertiCoq Require Import Block.vst.spec.spec.
+
+Lemma body: semax_body Vprog ASI f_certicoq_block__field_iter certicoq_block__field_iter_spec.
+Proof.
+  start_function.
+  forward_call.
+  admit.
+Admitted.
